src/QUIC.Parse.fst
@@ -662,10 +662,266 @@ let lemma_header_parsing_safe
 
 #pop-options
 
+module Impl = QUIC.Impl.Base
+
+inline_for_extraction
+noextract
+let destr_first_byte
+: (destr_bitsum'_t first_byte)
+= norm [primops; iota; zeta; delta_attr [`%filter_bitsum'_t_attr]]
+  (mk_destr_bitsum'_t first_byte)
+
+inline_for_extraction
+noextract
+let read_header_body_t
+  (sl: LL.slice (B.trivial_preorder _) (B.trivial_preorder _))
+  (cid_len: U32.t { U32.v cid_len < 20 } )
+  (last: uint62_t { U64.v last + 1 < pow2 62 })
+  (tg: bitsum'_type first_byte)
+: Tot (Type u#0)
+= (len: U32.t) ->
+  HST.Stack Impl.header
+  (requires (fun h ->
+    let p = dsnd (parse_header_body cid_len last (bitsum'_key_of_t first_byte tg)) in
+    LL.valid_pos (lp_parse_header cid_len last) h sl 0ul len /\
+    1 <= U32.v sl.LL.len /\
+    LL.valid_pos p h sl 1ul len /\
+    LL.contents (lp_parse_header cid_len last) h sl 0ul == (header_synth cid_len last).f tg (LL.contents p h sl 1ul)
+  ))
+  (ensures (fun h x h' ->
+    B.modifies B.loc_none h h' /\
+    begin
+      let hd = LL.contents (lp_parse_header cid_len last) h sl 0ul in
+      Impl.header_live x h' /\
+      LL.loc_slice_from_to sl 0ul len `B.loc_includes` Impl.header_footprint x /\
+      Impl.g_header x h' == hd
+    end
+  ))
+
+#push-options "--z3rlimit 64 --z3cliopt smt.arith.nl=false --using_facts_from '*,-FStar.Int.Cast' --query_stats --max_fuel 9 --initial_fuel 9 --max_ifuel 9 --initial_ifuel 9 --query_stats"
+
+inline_for_extraction
+noextract
+let read_header_body_short
+  (sl: LL.slice (B.trivial_preorder _) (B.trivial_preorder _))
+  (cid_len: U32.t { U32.v cid_len < 20 } )
+  (last: uint62_t { U64.v last + 1 < pow2 62 })
+  (spin: BF.bitfield uint8 1)
+  (key_phase: BF.bitfield uint8 1)
+  (pn_length: packet_number_length_t)
+: Tot (read_header_body_t sl cid_len last (| Short, (| (), (spin, (| (), (key_phase, (| pn_length, () |) ) |) ) |) |) )
+= fun len ->
+    let h0 = HST.get () in
+    assert_norm (bitsum'_key_of_t first_byte (| Short, (| (), (spin, (| (), (key_phase, (| pn_length, () |) ) |) ) |) |) == (| Short, (| (), (| (), (| pn_length, () |) |) |) |) );
+    LL.valid_nondep_then h0 (weaken (strong_parser_kind 0 20 None) (parse_flbytes (U32.v cid_len))) (parse_packet_number last pn_length) sl 1ul;
+    LL.valid_weaken (strong_parser_kind 0 20 None) (parse_flbytes (U32.v cid_len)) h0 sl 1ul;
+    LB.valid_flbytes_elim h0 (U32.v cid_len) sl 1ul;
+    let pos = LB.jump_flbytes (U32.v cid_len) cid_len sl 1ul in
+    let dcid = B.sub sl.LL.base 1ul (pos `U32.sub` 1ul) in
+    let pn = read_packet_number last pn_length sl pos in
+    Impl.BShort (spin = 1uy) (key_phase = 1uy) dcid cid_len pn pn_length
+
+#pop-options
+
+#push-options "--z3rlimit 128 --z3cliopt smt.arith.nl=false --using_facts_from '*,-FStar.Int.Cast' --query_stats --max_fuel 9 --initial_fuel 9 --max_ifuel 9 --initial_ifuel 9 --query_stats"
+
+#restart-solver
+
+inline_for_extraction
+noextract
+let read_header_body_long_retry
+  (sl: LL.slice (B.trivial_preorder _) (B.trivial_preorder _))
+  (cid_len: U32.t { U32.v cid_len < 20 } )
+  (last: uint62_t { U64.v last + 1 < pow2 62 })
+  (unused: BF.bitfield uint8 4)
+: Tot (read_header_body_t sl cid_len last (| Long, (| (), (| Retry, (unused, ()) |) |) |) )
+= fun len ->
+    let h0 = HST.get () in
+    assert_norm (bitsum'_key_of_t first_byte (| Long, (| (), (| Retry, (unused, ()) |) |) |)  == (| Long, (| (), (| Retry, () |) |) |) );
+    LL.valid_nondep_then h0 parse_common_long (parse_bounded_vlbytes 0 20) sl 1ul;
+    LL.valid_nondep_then h0 parse_u32 (parse_bounded_vlbytes 0 20 `nondep_then` parse_bounded_vlbytes 0 20) sl 1ul;
+    let version = LJ.read_u32 sl 1ul in
+    let pos1 = LJ.jump_u32 sl 1ul in
+    LL.valid_nondep_then h0 (parse_bounded_vlbytes 0 20) (parse_bounded_vlbytes 0 20) sl pos1;
+    let dcid = LB.get_vlbytes_contents 0 20 sl pos1 in
+    let dcid_len = LB.bounded_vlbytes_payload_length 0 20 sl pos1 in
+    let pos2 = LB.jump_bounded_vlbytes 0 20 sl pos1 in
+    let scid = LB.get_vlbytes_contents 0 20 sl pos2 in
+    let scid_len = LB.bounded_vlbytes_payload_length 0 20 sl pos2 in
+    let pos3 = LB.jump_bounded_vlbytes 0 20 sl pos2 in
+    let odcid = LB.get_vlbytes_contents 0 20 sl pos3 in
+    let odcid_len = LB.bounded_vlbytes_payload_length 0 20 sl pos3 in
+    Impl.BLong version dcid dcid_len scid scid_len (Impl.BRetry unused odcid odcid_len)
+
+#pop-options
+
+#push-options "--z3rlimit 512 --z3cliopt smt.arith.nl=false --using_facts_from '*,-FStar.Int.Cast' --query_stats --max_fuel 9 --initial_fuel 9 --max_ifuel 9 --initial_ifuel 9 --query_stats"
+
+#restart-solver
+
+inline_for_extraction
+noextract
+let read_header_body_long_initial
+  (sl: LL.slice (B.trivial_preorder _) (B.trivial_preorder _))
+  (cid_len: U32.t { U32.v cid_len < 20 } )
+  (last: uint62_t { U64.v last + 1 < pow2 62 })
+  (pn_length: packet_number_length_t)
+: Tot (read_header_body_t sl cid_len last (| Long, (| (), (| Initial, (| (), (| pn_length, () |) |) |) |) |) )
+= fun len ->
+    let h0 = HST.get () in
+    assert_norm (bitsum'_key_of_t first_byte (| Long, (| (), (| Initial, (| (), (| pn_length, () |) |) |) |) |) == (| Long, (| (), (| Initial, (| (), (| pn_length, () |) |) |) |) |) );
+    LL.valid_nondep_then h0 parse_common_long (parse_bounded_vlgenbytes 0 token_max_len (parse_bounded_varint 0 token_max_len) `nondep_then` parse_payload_length_pn last pn_length) sl 1ul;
+    LL.valid_nondep_then h0 parse_u32 (parse_bounded_vlbytes 0 20 `nondep_then` parse_bounded_vlbytes 0 20) sl 1ul;
+    let version = LJ.read_u32 sl 1ul in
+    let pos1 = LJ.jump_u32 sl 1ul in
+    LL.valid_nondep_then h0 (parse_bounded_vlbytes 0 20) (parse_bounded_vlbytes 0 20) sl pos1;
+    let dcid = LB.get_vlbytes_contents 0 20 sl pos1 in
+    let dcid_len = LB.bounded_vlbytes_payload_length 0 20 sl pos1 in
+    let pos2 = LB.jump_bounded_vlbytes 0 20 sl pos1 in
+    let scid = LB.get_vlbytes_contents 0 20 sl pos2 in
+    let scid_len = LB.bounded_vlbytes_payload_length 0 20 sl pos2 in
+    let pos3 = LB.jump_bounded_vlbytes 0 20 sl pos2 in
+    LL.valid_nondep_then h0 (parse_bounded_vlgenbytes 0 token_max_len (parse_bounded_varint 0 token_max_len)) (parse_payload_length_pn last pn_length) sl pos3;
+    let token = LB.get_bounded_vlgenbytes_contents 0 token_max_len (read_bounded_varint 0 token_max_len) (jump_bounded_varint 0 token_max_len) sl pos3 in
+    let token_len = LB.bounded_vlgenbytes_payload_length 0 token_max_len (read_bounded_varint 0 token_max_len) sl pos3 in
+    let pos4 = LB.jump_bounded_vlgenbytes 0 token_max_len (jump_bounded_varint 0 token_max_len) (read_bounded_varint 0 token_max_len) sl pos3 in
+    LL.valid_nondep_then h0 parse_varint (parse_packet_number last pn_length) sl pos4;
+    let payload_length = read_varint sl pos4 in
+    let pos5 = jump_varint sl pos4 in
+    let pn = read_packet_number last pn_length sl pos5 in
+//    assert (LL.loc_slice_from_to sl 0ul len `B.loc_includes` B.loc_buffer token);
+    Impl.BLong version dcid dcid_len scid scid_len (Impl.BInitial payload_length pn pn_length token token_len)
+
+#pop-options
+
+#push-options "--z3rlimit 128 --z3cliopt smt.arith.nl=false --using_facts_from '*,-FStar.Int.Cast' --query_stats --max_fuel 9 --initial_fuel 9 --max_ifuel 9 --initial_ifuel 9 --query_stats"
+
+#restart-solver
+
+inline_for_extraction
+noextract
+let read_header_body_long_handshake
+  (sl: LL.slice (B.trivial_preorder _) (B.trivial_preorder _))
+  (cid_len: U32.t { U32.v cid_len < 20 } )
+  (last: uint62_t { U64.v last + 1 < pow2 62 })
+  (pn_length: packet_number_length_t)
+: Tot (read_header_body_t sl cid_len last (| Long, (| (), (| Handshake, (| (), (| pn_length, () |) |) |) |) |) )
+= fun len ->
+    let h0 = HST.get () in
+    assert_norm (bitsum'_key_of_t first_byte (| Long, (| (), (| Handshake, (| (), (| pn_length, () |) |) |) |) |) == (| Long, (| (), (| Handshake, (| (), (| pn_length, () |) |) |) |) |) );
+    LL.valid_nondep_then h0 parse_common_long (parse_payload_length_pn last pn_length) sl 1ul;
+    LL.valid_nondep_then h0 parse_u32 (parse_bounded_vlbytes 0 20 `nondep_then` parse_bounded_vlbytes 0 20) sl 1ul;
+    let version = LJ.read_u32 sl 1ul in
+    let pos1 = LJ.jump_u32 sl 1ul in
+    LL.valid_nondep_then h0 (parse_bounded_vlbytes 0 20) (parse_bounded_vlbytes 0 20) sl pos1;
+    let dcid = LB.get_vlbytes_contents 0 20 sl pos1 in
+    let dcid_len = LB.bounded_vlbytes_payload_length 0 20 sl pos1 in
+    let pos2 = LB.jump_bounded_vlbytes 0 20 sl pos1 in
+    let scid = LB.get_vlbytes_contents 0 20 sl pos2 in
+    let scid_len = LB.bounded_vlbytes_payload_length 0 20 sl pos2 in
+    let pos3 = LB.jump_bounded_vlbytes 0 20 sl pos2 in
+    LL.valid_nondep_then h0 parse_varint (parse_packet_number last pn_length) sl pos3;
+    let payload_length = read_varint sl pos3 in
+    let pos4 = jump_varint sl pos3 in
+    let pn = read_packet_number last pn_length sl pos4 in
+    Impl.BLong version dcid dcid_len scid scid_len (Impl.BHandshake payload_length pn pn_length)
+
+#restart-solver
+
+inline_for_extraction
+noextract
+let read_header_body_long_ZeroRTT
+  (sl: LL.slice (B.trivial_preorder _) (B.trivial_preorder _))
+  (cid_len: U32.t { U32.v cid_len < 20 } )
+  (last: uint62_t { U64.v last + 1 < pow2 62 })
+  (pn_length: packet_number_length_t)
+: Tot (read_header_body_t sl cid_len last (| Long, (| (), (| ZeroRTT, (| (), (| pn_length, () |) |) |) |) |) )
+= fun len ->
+    let h0 = HST.get () in
+    assert_norm (bitsum'_key_of_t first_byte (| Long, (| (), (| ZeroRTT, (| (), (| pn_length, () |) |) |) |) |) == (| Long, (| (), (| ZeroRTT, (| (), (| pn_length, () |) |) |) |) |) );
+    LL.valid_nondep_then h0 parse_common_long (parse_payload_length_pn last pn_length) sl 1ul;
+    LL.valid_nondep_then h0 parse_u32 (parse_bounded_vlbytes 0 20 `nondep_then` parse_bounded_vlbytes 0 20) sl 1ul;
+    let version = LJ.read_u32 sl 1ul in
+    let pos1 = LJ.jump_u32 sl 1ul in
+    LL.valid_nondep_then h0 (parse_bounded_vlbytes 0 20) (parse_bounded_vlbytes 0 20) sl pos1;
+    let dcid = LB.get_vlbytes_contents 0 20 sl pos1 in
+    let dcid_len = LB.bounded_vlbytes_payload_length 0 20 sl pos1 in
+    let pos2 = LB.jump_bounded_vlbytes 0 20 sl pos1 in
+    let scid = LB.get_vlbytes_contents 0 20 sl pos2 in
+    let scid_len = LB.bounded_vlbytes_payload_length 0 20 sl pos2 in
+    let pos3 = LB.jump_bounded_vlbytes 0 20 sl pos2 in
+    LL.valid_nondep_then h0 parse_varint (parse_packet_number last pn_length) sl pos3;
+    let payload_length = read_varint sl pos3 in
+    let pos4 = jump_varint sl pos3 in
+    let pn = read_packet_number last pn_length sl pos4 in
+    Impl.BLong version dcid dcid_len scid scid_len (Impl.BZeroRTT payload_length pn pn_length)
+
+inline_for_extraction
+noextract
+let read_header_body
+  (sl: LL.slice (B.trivial_preorder _) (B.trivial_preorder _))
+  (cid_len: U32.t { U32.v cid_len < 20 } )
+  (last: uint62_t { U64.v last + 1 < pow2 62 })
+  (tg: bitsum'_type first_byte)
+: Tot (read_header_body_t sl cid_len last tg)
+= fun len ->
+  let h0 = HST.get () in
+  match tg with
+  | (| Short, (| (), (spin, (| (), (key_phase, (| pn_length, () |) ) |) ) |) |) ->
+    read_header_body_short sl cid_len last spin key_phase pn_length len
+  | (| Long, (| (), (| Retry, (unused, ()) |) |) |) ->
+    read_header_body_long_retry sl cid_len last unused len
+  | (| Long, (| (), (| Initial, (| (), (| pn_length, () |) |) |) |) |) ->
+    read_header_body_long_initial sl cid_len last pn_length len
+  | (| Long, (| (), (| Handshake, (| (), (| pn_length, () |) |) |) |) |) ->
+    read_header_body_long_handshake sl cid_len last pn_length len
+  | (| Long, (| (), (| ZeroRTT, (| (), (| pn_length, () |) |) |) |) |) ->
+    read_header_body_long_ZeroRTT sl cid_len last pn_length len
+
+#pop-options
+
+#restart-solver
+
+#push-options "--z3rlimit 64 --z3cliopt smt.arith.nl=false --using_facts_from '*,-FStar.Int.Cast' --query_stats"
+
 let read_header
   packet packet_len cid_len last
 =
-  admit ()
+  let h0 = HST.get () in
+  let sl = LL.make_slice packet packet_len in
+  LL.valid_facts (lp_parse_header cid_len last) h0 sl 0ul;
+  assert (B.as_seq h0 packet `Seq.equal` LL.bytes_of_slice_from h0 sl 0ul);
+  let len = validate_header cid_len last sl 0ul in
+  if len `U32.gt` LL.validator_max_length
+  then None
+  else begin
+    let g = Ghost.hide (LL.contents (lp_parse_header cid_len last) h0 sl 0ul) in
+    LL.valid_bitsum_elim
+      #parse_u8_kind
+      #8
+      #U8.t
+      #uint8
+      first_byte
+      #(header' cid_len last)
+      (first_byte_of_header cid_len last)
+      (header_body_type cid_len last)
+      (header_synth cid_len last)
+      parse_u8
+      (parse_header_body cid_len last)
+      h0
+      sl
+      0ul;
+    let r = LJ.read_u8 sl 0ul in
+    let res = destr_first_byte
+      (read_header_body_t sl cid_len last)
+      (fun _ cond dt df len' -> if cond then dt () len' else df () len')
+      (read_header_body sl cid_len last)
+      r
+      len
+    in
+    lemma_header_parsing_post (U32.v cid_len) (U64.v last) (LL.bytes_of_slice_from h0 sl 0ul);
+    Some (res, len)
+  end
 
 let impl_header_length
   x
@@ -676,3 +932,5 @@ let write_header
   dst x
 =
   admit ()
+
+#pop-options
