src/QUIC.Parse.PacketNumber.fsti
@@ -31,7 +31,20 @@ val serialize_packet_number
   (pn_len: packet_number_length_t)
 : Tot (serializer (parse_packet_number last pn_len))
 
+inline_for_extraction
 val validate_packet_number
   (last: last_packet_number_t)
   (pn_len: packet_number_length_t)
 : Tot (validator (parse_packet_number last pn_len))
+
+inline_for_extraction
+val jump_packet_number
+  (last: last_packet_number_t)
+  (pn_len: packet_number_length_t)
+: Tot (jumper (parse_packet_number last pn_len))
+
+inline_for_extraction
+val read_packet_number
+  (last: last_packet_number_t)
+  (pn_len: packet_number_length_t)
+: Tot (leaf_reader (parse_packet_number last pn_len))
